\subsection{The Substitution Rule}
In general, suppose we have an integral of the form
\[\int f(g(x))g'(x)\,dx\]
Observe that if \(F'=f\), then
\[\int F'(g(x))g'(x)\,dx=F(g(x))+C\]
because, by the Chain Rule,
\[\frac{d}{dx}\big[F(g(x))\big]=F'(g(x))\cdot g'(x)\]
If we make the ``change of variable'' or ``substitution'' \(u=g(x)\), then we
have
\[\int F'(g(x)g'(x)\,dx=F(g(x)))+C=F(u)+C=\int F'(u)\,du\]
or, writing \(F'=f\), we get
\[\int f(g(x))g'(x)\,dx=\int f(u)\,du\]
Thus we proved the following rule. \\
\textbf{The Substitution Rule}: If \(u=g(x)\) is a differentiable function
whose range is an interval \(I\) and \(f\) is continuous on \(I\), then
\[\int f(g(x))g'(x)\,dx=\int f(u)\,du\]
Notice that if \(u=g(x)\), then \(du=g'(x)\,dx\).
It is permissible to operate with \(dx\) and \(du\) after integral signs as if
they were differentials.

\begin{problem}
    Evaluate \(\displaystyle{\int\frac{x}{\sqrt{1-4x^2}}\,dx}\).
\end{problem}
\begin{solution}
    Let \(u=1-4x^2\iff du=-8x\,dx\) so \(xdx=-\dfrac{1}{8}\,du\).
    Therefore,
    \[\int\frac{x}{\sqrt{1-4x^2}}\,dx=-\int\frac{1}{8}u^{-(1/2)}\,du
    =-\frac{1}{8}(2\sqrt{u})+C=-\frac{1}{4}\sqrt{1-4x^2}+C\]
\end{solution}
\begin{problem}
    Evaluate \(\displaystyle{\int\tan x\,dx}\).
\end{problem}
\begin{solution}
    We have \(\displaystyle{\int\tan x\,dx=\int\frac{\sin x}{\cos x}}\,dx\),
    let \(u=\cos x \iff du=-\sin\,dx\) then
    \[\int\tan x\,dx=-\int\frac{du}{u}=-\ln|u|+C=-\ln|\cos x|+C
    =\ln\frac{1}{|\sec x|}+C=\ln|\sec x|+C\]
\end{solution}

\subsubsection*{Definite Integrals}
\textbf{The Substitution Rule for Definite Integrals}: If \(g'\) is continuous
on \([a,b]\) and \(f\) is continuous on the range of \(u=g(x)\), then
\[\int_a^b f(g(x))g'(x)\,dx=\int_{g(a)}^{g(b)}f(u)\,du\]
Note that we must change the limits of integration when the variable is
changed for definite integrals.
\begin{proof}
    Let \(F\) be an antiderivative of \(f\).
    Then \(F(g(x))\) is an antiderivative of \(f(g(x))g'(x)\) and so, by the
    Fundamental Theorem of Calculus, we have
    \[\int_a^b f(g(x))g'(x)\,dx=F(g(b))-F(g(a))\]
    But, applying the Fundamental Theorem of Calculus a second time, we also
    have
    \[\int_{g(a)}^{g(b)}\int f(u)\,du=\big[F(u)\big]_{g(a)}^{g(b)}
    =F(g(b))-F(g(a))\]
\end{proof}
\begin{problem}
    Calculate \(\displaystyle{\int_1^e \frac{\ln x}{x}\,dx}\).
\end{problem}
\begin{solution}
    Let \(u=\ln x\iff du=\dfrac{1}{x}\,dx\), then
    \[\int_1^e \frac{\ln x}{x}\,dx=\int_0^1 u\,du
    =\left[\frac{u^2}{2}\right]_0^1=\frac{1}{2}\]
\end{solution}

\subsubsection*{Symmetry}
Integrals of Symmetric Functions: Suppose \(f\) is continuous on \([-a,a]\).
\begin{enumerate}
    \item If \(f\) is even, then
    \(\displaystyle{\int_{-a}^a f(x)\,dx}=2\int_0^a f(x)\,dx\).
    \item If \(f\) is odd, then \(\displaystyle{\int_{-a}^a f(x)\,dx=0}\).
\end{enumerate}
\begin{proof}
    We split the integral in two:
    \[\int_{-a}^a f(x)\,dx=\int_{-a}^0 f(x)\,dx+\int_0^a f(x)\,dx
    =-\int_0^{-a}f(x)\,dx+\int_0^a f(x)\,dx\]
    We make the substitution \(u=-x\).
    Then \(du=-dx\) and when \(x=-a,u=a\).
    Therefore
    \[-\int_0^{-a}f(x)\,dx=-\int_0^a f(-u)(-du)=\int_0^a f(-u)\,du\]
    and so
    \[\int_{-a}^a f(x)\,dx=\int_0^a f(-u)\,du+\int_0^a f(x)\,dx\]
    \begin{enumerate}
        \item If \(f\) is even, then \(f(-u)=f(u)\) so
        \[\int_{-a}^a f(x)\,dx=\int_0^a f(u)\,du+\int_0^a f(x)\,dx
        =2\int_0^a f(x)\,dx\]
        \item If \(f\) is odd, then \(f(-u)=-f(u)\) so
        \[\int_{-a}^a f(x)\,dx=-\int_0^a f(u)\,du+\int_0^a f(x)\,dx=0\]
    \end{enumerate}
\end{proof}