\subsection{Trigonometric Integrals and Substitutions}
\subsubsection{Trigonometric Integrals}
We can use trigonometric identities to integrate trigonometric integrals.
\begin{problem}
    Evaluate \(\displaystyle{\int\cos^3 x\,dx}\).
\end{problem}
\begin{solution}
    \[\int\cos^3 x\,dx=\int(1-\sin^2 x)\cos x\,dx=\int(1-u^2)\,du
    =u-\frac{u^3}{3}+C=\sin x-\frac{1}{3}\sin^3 x+C\qedhere\]
\end{solution}
\begin{problem}
    Evaluate \(\displaystyle{\int\sin^5 x\cos^2 x\,dx}\).
\end{problem}
\begin{solution}
    \begin{align*}
        \int\sin^5 x\cos^2 x\,dx &= \int(1-\cos^2 x)^2\cos^2 x\sin x\,dx
        =-\int(1-u^2)^2u^2\,du \\
        &= -\int(u^2-2u^4+u^6)\,du
        =-\frac{1}{3}u^3+\frac{2}{5}u^5-\frac{1}{7}u^7+C \\
        &= -\frac{1}{3}\cos^3 x+\frac{2}{5}\cos^5 x-\frac{1}{7}\cos^7 x
        +C \qedhere
    \end{align*}
\end{solution}
\begin{problem}
    Evaluate \(\displaystyle{\int\cos^2 x\,dx}\).
\end{problem}
\begin{solution}
    \[\int\cos^2 x\,dx=\int\frac{1}{2}(1+\cos 2x)\,dx
    =\frac{1}{2}\left(\int dx+\int\cos 2x\,dx\right)
    =\frac{1}{2}\left(x+\frac{1}{2}\sin 2x\right)+C\qedhere\]
\end{solution}
\begin{problem}
    Evaluate \(\displaystyle{\int_0^\pi\sin^2 x\,dx}\).
\end{problem}
\begin{solution}
    \begin{align*}
    \int_0^\pi\sin^2 x\,dx &= \int_0^\pi\frac{1}{2}(1-\cos 2x)\,dx
    =\frac{1}{2}\left(\int_0^\pi dx-\int_0^\pi\cos 2x\,dx\right) \\
    &=\frac{1}{2}
    \left(\bigl[x\bigr]_0^\pi-\frac{1}{2}\bigl[\sin 2x\bigr]_0^\pi\right)
    =\frac{\pi}{2} \qedhere
    \end{align*}
\end{solution}
\begin{problem}
    Evaluate \(\displaystyle{\int\sin^4 x\,dx}\).
\end{problem}
\begin{solution}
    \begin{align*}
        \int\sin^4 x\,dx &= \int\left(\frac{1}{2}(1-\cos 2x)\right)^2\,dx
        =\frac{1}{4}\int(1-2\cos 2x+\cos^2 2x)\,dx \\
        &= \frac{1}{4}
        \left(x-\sin 2x+\frac{1}{2}
        \left(x+\frac{1}{4}\sin 4x\right)\right)+C \\
        &= \frac{1}{4}
        \left(\frac{3}{2}x-\sin 2x+\frac{1}{8}\sin 4x\right)+C \qedhere
    \end{align*}
\end{solution}
In general, an integral of powers of \(\sin x\) and \(\cos x\) is in the
form
\[\int\sin^m x\cos^n x\,dx\]
where \(m,n\in\Z\) and \(m,n\geq 0\).
If \(m\) is odd, then we save a factor \(\sin x\) and express the rest to
terms in \(\cos x\) for substitution.
If \(n\) is odd, then we save a factor \(\cos x\) and express the rest to
terms in \(\sin x\) for substitution.
If \(m\) and \(n\) are even, then we use the power reduction formulas.
\begin{problem}
    Evaluate \(\displaystyle{\int\tan^6 x\sec^4 x\,dx}\).
\end{problem}
\begin{solution}
    \begin{align*}
        \int\tan^6 x\sec^4 x\,dx &= \int\tan^6 x(\tan^2 x+1)\sec^2 x\,dx
        =\int u^6(u^2+1)\,du=\int u^8+u^6 \\
        & =\frac{u^9}{9}+\frac{u^7}{7}
        =\frac{1}{9}\tan^9 x+\frac{1}{7}\tan^7 x+C \qedhere
    \end{align*}
\end{solution}
\begin{problem}
    Evaluate \(\displaystyle{\int\tan^5 x\sec^7 x\,dx}\).
\end{problem}
\begin{solution}
    \begin{align*}
        \int\tan^5 x\sec^7 x\,dx
        &= \int(\sec^2 x-1)^2\sec^6 x\sec x\tan x\,dx
        =\int(u^2-1)^2u^6\,du \\
        &= \int(u^{10}-2u^8+u^6)\,dx
        =\frac{1}{11}u^{11}-\frac{2}{9}u^9+\frac{1}{7}u^7+C \\
        &= \frac{1}{11}\sec^{11}x-\frac{2}{9}\sec^9 x+\frac{1}{7}\sec^7 x
        +C \qedhere
    \end{align*}
\end{solution}
In general, an integral of powers of \(\tan x\) and \(\sec x\) is in the
form
\[\int\tan^m x\sec^n x\,dx\]
where \(m,n\in\Z\) and \(m,n\geq 0\).
If \(m\) is odd, then we save a factor of \(\sec x\tan x\) and express the
rest in terms of \(\sec x\) for substitution.
If \(n\) is even, then we save a factor of \(\sec^2 x\) and express the
rest in terms of \(\tan x\) for substitution.
\begin{problem}
    Evaluate \(\displaystyle{\int\sec x\,dx}\).
\end{problem}
\begin{solution}
    We have
    \[\int\sec x\,dx=\int\sec x\frac{\sec x+\tan x}{\sec x+\tan x}\,dx
    =\int\frac{\sec^2 x+\sec x\tan x}{\sec x+\tan x}\,dx\]
    Let \(u=\sec x+\tan x\iff du=(\sec x\tan x+\sec^2 x)\,dx\), then
    \[\int\sec x\,dx=\int\frac{\sec^2 x+\sec x\tan x}{\sec x+\tan x}\,dx
    =\int\frac{du}{u}=\ln|u|+C=\ln|\sec x+\tan x|+C\qedhere\]
\end{solution}
The formula \(\displaystyle{\int\sec x\,dx=\ln|\sec x+\tan x|+C}\) was
discovered by James Gregory in 1668.
\begin{problem}
    Evaluate \(\displaystyle{\int\tan^3 x\,dx}\).
\end{problem}
\begin{solution}
    \begin{align*}
    \int\tan^3 x\,dx &= \int\tan x(\sec^2x-1)\,dx
    =\int\tan x\sec^2\,dx-\int\tan x\,dx \\
    &= \frac{1}{2}\tan^2 x-\ln|\sec x|+C \qedhere
    \end{align*}
\end{solution}
\begin{problem}
    Evaluate \(\displaystyle{\int\sec^3 x\,dx}\).
\end{problem}
\begin{solution}
    Let \(u=\sec x\iff du=\sec x\tan x\) and \(dv=\sec^2 x\,dx\iff v=\tan x\),
    then
    \[\int\sec^3 x\,dx=\sec x\tan x-\int\tan^2 x\sec x\,dx\]
    We have
    \[\int\tan^2 x\sec x\,dx=\int(\sec^2 x-1)\sec x\,dx
    =\int\sec^3 x\,dx-\int\sec x\,dx\]
    Therefore,
    \begin{align*}
        \int\sec^3 x\,dx &= \sec x\tan x-\int\sec^3 x\,dx+\int\sec x\,dx \\
        \int\sec^3 x\,dx
        &= \frac{1}{2}(\sec x\tan x+\ln|\sec x+\tan x|)+C \qedhere
    \end{align*}
\end{solution}

\subsubsection{Trigonometric Substitutions}
If an integral has the form \(\displaystyle{\int\sqrt{a^2-x^2}\,dx}\),
then we can use the substitution \(x=a\sin\theta\) where
\(-(\pi/2)\leq\theta\leq\pi/2\) to get
\[\sqrt{a^2-x^2}=\sqrt{a^2-a^2\sin^2\theta}=\sqrt{a^2(1-\sin^2\theta)}
=\sqrt{a^2\cos^2\theta}=|a|\cos\theta\]
If an integral has the form \(\displaystyle{\int\sqrt{a^2+x^2}\,dx}\),
then we can use the substitution \(x=a\tan\theta\) where
\(-(\pi/2)<\theta<\pi/2\) to get
\[\sqrt{a^2+x^2}=\sqrt{a^2+a^2\tan^2\theta}=\sqrt{a^2(\tan^2\theta+1)}
=\sqrt{a^2\sec^2\theta}=|a|\sec\theta\]
If an integral has the form \(\displaystyle{\int\sqrt{x^2-a^2}\,dx}\),
then we can use the substitution \(x=a\sec\theta\) where
\(0\leq\theta<\pi/2\) or \(\pi\leq\theta<3\pi/2\) to get
\[\sqrt{x^2-a^2}=\sqrt{a^2\sec^2\theta-a^2}=\sqrt{a^2(\sec^2\theta-1)}
=\sqrt{a^2\tan^2\theta}=|a|\tan\theta\]
\begin{problem}
    Evaluate \(\displaystyle{\int\frac{\sqrt{9-x^2}}{x^2}\,dx}\)
\end{problem}
\begin{solution}
    Let \(x=3\sin\theta\iff dx=3\cos\theta\,d\theta\), then
    \begin{align*}
    \int\frac{\sqrt{9-x^2}}{x^2}\,dx
    &= \int\frac{3\cos\theta}{9\sin^2\theta}3\cos\theta\,d\theta
    =\int\frac{\cos^2\theta}{\sin^2\theta}=\int\cot^2\theta\,d\theta
    =\int(\csc^2\theta-1)\,d\theta \\
    &=-\cot\theta-\theta+C
    =-\frac{\sqrt{9-x^2}}{x}-\arcsin\left(\frac{x}{3}\right)+C \qedhere
    \end{align*}
\end{solution}