\subsection{Hyperbolic Functions}

Definition of \textbf{hyperbolic functions}:
\begin{align*}
    \sinh x &= \frac{e^x-e^{-x}}{2} & \csch x &= \frac{1}{\sinh x} \\
    \cosh x &= \frac{e^x+e^{-x}}{2} & \sech x &= \frac{1}{\cosh x} \\
    \tanh x &= \frac{\sinh x}{\cosh x} & \coth x &= \frac{\cosh x}{\sinh x}
\end{align*}
Hyperbolic Identities:
\begin{itemize}
    \item \(\sinh(-x)=-\sinh x\)
    \item \(\cosh(-x)=\cosh x\)
    \item \(\cosh^2 x-\sinh^2 x=1\)
    \item \(1-\tanh^2 x=\sech^2 x\)
    \item \(\sinh(x+y)=\sinh x\cosh x+\cosh x\sinh y\)
    \item \(\cosh(x+y)=\cosh x\cosh x+\sinh x\sinh y\)
\end{itemize}
Derivatives of hyperbolic functions:
\begin{align*}
    \frac{d}{dx}(\sinh x) &= \cosh x
    & \frac{d}{dx}(\csch x) &= -\csch x\coth x \\
    \frac{d}{dx}(\cosh x) &= \sinh x
    & \frac{d}{dx}(\sech x) &= -\sech x\tanh x \\
    \frac{d}{dx}(\tanh x) &= \sech^2 x
    & \frac{d}{dx}(\coth x) &= -\csch^2 x
\end{align*}

\subsubsection*{Inverse Hyperbolic Functions}
\begin{align*}
    \arsinh x &= \ln(x+\sqrt{x^2+1}),\quad x\in\R \\
    \arcosh x &= \ln(x+\sqrt{x^2-1}),\quad x\geq 1 \\
    \artanh x &= \frac{1}{2}\ln\left(\frac{1+x}{1-x}\right),
    \quad -1\leq x\leq 1
\end{align*}
Derivatives of inverse hyperbolic functions:
\begin{align*}
    \frac{d}{dx}(\arsinh x) &= \frac{1}{\sqrt{1+x^2}}
    & \frac{d}{dx}(\arcsch x) &= -\frac{1}{|x|\sqrt{x^2+1}} \\
    \frac{d}{dx}(\arcosh x) &= \frac{1}{\sqrt{x^2-1}}
    & \frac{d}{dx}(\arsech x) &= -\frac{1}{x\sqrt{1-x^2}} \\
    \frac{d}{dx}(\artanh x) &= \frac{1}{1-x^2}
    & \frac{d}{dx}(\arcoth x) &= \frac{1}{1-x^2}
\end{align*}