\subsection{Implicit Differentiation}
An \textbf{explicit function} \(y=f(x)\) is defined by expressing one variable
explicitly in terms of another variable.
An \textbf{implicit function} is defined implicitly by a relation between
\(x\) and \(y\).
An example of implicit functions is the equation of the circle \(x^2+y^2=r^2\)
where the raidus \(r\) is a constant.
In some cases it is possible to solve an implicit function to get an explicit function.
We can use the method of \textbf{implicit differentiation} to find the derivative
of \(y\) in an implicit function.
\begin{problem}
    Find \(dy/dx\) of the unit circle \(x^2+y^2=1\).
\end{problem}
\begin{solution}
    We differentiate on both sides of the equation then we have
    \begin{align*}
        \frac{d}{dx}(x^2+y^2)&=\frac{d}{dx}(1)\\
        \frac{d}{dx}(x^2)+\frac{d}{dx}(y^2)&=0
    \end{align*}
    Since \(y=f(x)\), we use the chain rule then we have
    \begin{align*}
        2x+\frac{d}{dy}(y^2)\frac{dy}{dx}=0\\
        2x+2y\frac{dy}{dx}=0
    \end{align*}
    We solve for \(dy/dx\) then we have
    \[\frac{dy}{dx}=-\frac{x}{y}\qedhere\]
\end{solution}
\begin{problem}
    Find \(dy/dx\) of the folium of Descartes \(x^3+y^3=6xy\).
\end{problem}
\begin{solution}
    \begin{align*}
        x^3+y^3&=6xy\\\frac{d}{dx}x^3+\frac{d}{dy}y^3\left(\frac{dy}{dx}\right)
        &=\left[\frac{d}{dx}(6x)\right]y+6x\frac{dy}{dx}\\3x^2+3y^2\frac{dy}{dx}
        &=6y+6x\frac{dy}{dx}\\x^2+y^2\frac{dy}{dx}&=2y+2x\frac{dy}{dx}
        \\(y^2-2x)\frac{dy}{dx}&=2y-x^2\\\frac{dy}{dx}&=\frac{2y-x^2}{y^2-2x}\qedhere
    \end{align*}
\end{solution}