\subsection{Implicit Differentiation}

\subsubsection*{Implicit Differentiation}
An explicit function \(y=f(x)\) is defined by expressing one variable
explicitly in terms of another variable.
An implicit function is defined implicitly by a relation between \(x\) and
\(y\).
An example of implicit functions is the equation of the circle \(x^2+y^2=r^2\)
where the raidus \(r\) is a constant.
In some cases it is possible to solve an implicit function to get an explicit function.
We can use the method of \textbf{implicit differentiation} to find the derivative
of \(y\) in an implicit function.
\begin{problem}
    Find \(dy/dx\) of the unit circle \(x^2+y^2=1\).
\end{problem}
\begin{solution}
    We differentiate on both sides of the equation then we have
    \begin{align*}
        \frac{d}{dx}(x^2+y^2) &= \frac{d}{dx}(1) \\
        \frac{d}{dx}(x^2)+\frac{d}{dx}(y^2) &= 0
    \end{align*}
    Since \(y=f(x)\), we use the chain rule then we have
    \begin{align*}
        2x+\frac{d}{dy}(y^2)\frac{dy}{dx} &= 0 \\
        2x+2y\frac{dy}{dx} &= 0
    \end{align*}
    We solve for \(dy/dx\) then we have
    \[\frac{dy}{dx}=-\frac{x}{y}\]
\end{solution}
\begin{problem}
    Find \(dy/dx\) of the folium of Descartes \(x^3+y^3=6xy\).
\end{problem}
\begin{solution}
    \begin{align*}
        x^3+y^3 &= 6xy \\
        \frac{d}{dx}x^3+\frac{d}{dy}y^3\left(\frac{dy}{dx}\right)
        &= \left[\frac{d}{dx}(6x)\right]y+6x\frac{dy}{dx} \\
        3x^2+3y^2\frac{dy}{dx} &= 6y+6x\frac{dy}{dx} \\
        x^2+y^2\frac{dy}{dx} &= 2y+2x\frac{dy}{dx} \\
        (y^2-2x)\frac{dy}{dx} &= 2y-x^2 \\
        \frac{dy}{dx} &= \frac{2y-x^2}{y^2-2x} 
    \end{align*}
\end{solution}
\begin{problem}
    Find \(y'\) if \(\sin(x+y)=y^2\cos x\).
\end{problem}
\begin{solution}
    \begin{align*}
        \sin(x+y) &= y^2\cos x \\
        \cos(x+y)(1+\frac{dy}{dx}) &= 2y\frac{dy}{dx}\cos x-y^2\sin x \\
        [2y\cos x-\cos(x+y)]\frac{dy}{dx} &= \cos(x+y)+y^2\sin x \\
        \frac{dy}{dx}
        &= \frac{\cos(x+y)+y^2\sin x}{2y\cos x-\cos(x+y)} 
    \end{align*}
\end{solution}
\begin{problem}
    Find \(y''\) if \(x^4+y^4=16\).
\end{problem}
\begin{solution}
    First we find \(y'\) then we have
    \begin{align*}
        x^4+y^4 &= 16 \\ 4x^3+4y^3\frac{dy}{dx} &= 0 \\
        \frac{dy}{dx} &= -\frac{x^3}{y^3}
    \end{align*}
    Then we find \(y''\) and we have
    \begin{align*}
        \frac{d^2y}{dx^2} &= \frac{d}{dx}\left(-\frac{x^3}{y^3}\right)
        =-3x^2y^{-3}+(-x^3)(-3y^{-4})\frac{dy}{dx}
        =3x^3y^{-4}(-x^3y^{-3})-3x^2y^{-3} \\
        &= -3x^6y^{-7}-3x^2y^{-3}
        =-3x^2y^{-7}(x^4+y^4)=-48\frac{x^2}{y^7} 
    \end{align*}
\end{solution}